partialImpliesFull.v
@@ -1,5 +1,6 @@
 Require Export stepPreservesRewind.  
 
+(*
 (*if the endpoint of a replay derivation can be validated, then the 
 **start point can be validated too*)
 Theorem replayCommit : forall S L H L' S' H' e0 e e', 
@@ -16,56 +17,60 @@ Proof.
   }
 Qed. 
 
+
+ *)
+
 (*simulate a replay relation under full abort semantics as long as the endpoint
 **log is valid*)
-Theorem replayFMulti : forall H S C C' e0 L e L' S' e' H', 
-                         replay H (Some(S,e0),L,e) (Some(S,e0),L',e') ->
-                         validate S L' H S' (commit H') -> S < C ->
-                         f_multistep C' H (Single(Some(C,e0),L,e)) C' H 
+Theorem replayFMulti : forall H C e0 L e L' e' H', 
+                         replay H C (Some(C,e0),L,e) (Some(C,e0),L',e') ->
+                         validate L' H (commit H') -> 
+                         f_multistep C H (Single(Some(C,e0),L,e)) C H 
                                      (Single(Some(C,e0),L',e')). 
-Proof. 
-  intros. dependent induction H0. 
+Proof.
+  intros. dependent induction H0.  
   {constructor. }
-  {inv H0. 
-   {econstructor. eapply f_transStep. eapply t_readStep; eauto. omega. eauto. }
-   {eapply replayCommit in H1; eauto. invertHyp. inv H0. lookupSame. omega. }
-   {econstructor. eapply f_transStep. eapply t_readInDomainStep; eauto. eauto. }
-   {econstructor. eapply f_transStep. eapply t_writeStep; eauto. intros c. 
-    inv c. eauto. }
-   {econstructor. eapply f_transStep. eapply t_atomicIdemStep; eauto. intros c. 
-    inv c. eauto. }
-   {econstructor. eapply f_transStep. eapply t_betaStep; eauto. intros c. 
-    inv c. eauto. }
+  {inv H0.
+   {econstructor. eapply c_transStep. econstructor; eauto.
+    eapply IHreplay; eauto. }
+   {omega. }
+   {econstructor. eapply c_transStep. eapply t_readInDomainStep; eauto.
+    eapply IHreplay; eauto. }
+   {econstructor. eapply c_transStep. eapply t_writeStep; eauto.
+    eapply IHreplay; eauto. }
+   {econstructor. eapply c_transStep. eapply t_atomicIdemStep; eauto.
+    eapply IHreplay; eauto. }
+   {econstructor. eapply c_transStep. eapply t_betaStep; eauto.
+    eapply IHreplay; eauto. }
   }
 Qed. 
-
+                              
 (*full abort can simulate partial abort*)
 Theorem partialImpliesFull : forall C H T C' H' T', 
                                p_step C H T C' H' T' -> poolRewind C H T ->
                                f_multistep C H T C' H' T'. 
 Proof.
   intros. induction H0.
-  {econstructor. eapply f_transStep. eauto. constructor. }
-  {inv H1. apply IHp_step in H4. apply f_multi_L. auto. }
-  {inv H1. apply IHp_step in H5. apply f_multi_R. auto. }
-  {inv H1. econstructor. eapply f_forkStep; eauto. constructor. }
-  {inv H3. 
-   {copy H12. inv H1. eapply abortRewind in H12; eauto. copy H3. 
-    eapply validateValidate in H1. invertHyp. econstructor. 
-    eapply f_eagerAbort; eauto. econstructor. eauto. 
-    rewrite rewindIFFReplay in H12. eapply replayFMulti; eauto. }
-   {inv H1. econstructor. eapply f_eagerAbort; eauto.
-    eapply validateAbortRead; eauto. rewrite rewindIFFReplay in H7. 
-    eapply decomposeEq in H4. subst. eapply replayFMulti; eauto. }
+  {inv H0. econstructor. eapply c_liftedStep. econstructor.
+   eauto. inv H1. eapply rewindAbort in H2; eauto.
+   eapply validateValidate in H3. invertHyp.
+   eapply rewindNewerStamp in H2; eauto. eapply replayFMulti.
+   rewrite <- rewindIFFReplay. eauto. eauto. }
+  {inv H0.
+   {econstructor. eapply c_transStep. econstructor; eauto. constructor. }
+   {econstructor. eapply c_transStep. econstructor; eauto. constructor. }
+   {econstructor. eapply c_transStep. econstructor; eauto. constructor. }
+   {econstructor. eapply c_transStep. eapply t_atomicIdemStep; eauto. constructor. }
+   {econstructor. eapply c_transStep. eapply t_betaStep; eauto. constructor. }
   }
-  {inv H1. copy H0. eapply abortRewind in H1; eauto. copy H0. 
-   eapply validateValidate in H2. invertHyp. econstructor. 
-   eapply f_abortStep; eauto. rewrite rewindIFFReplay in H1. 
-   eapply replayFMulti; eauto. }
-  {econstructor. eapply f_allocStep; eauto. constructor. }
-  {econstructor. eapply f_commitStep; eauto. constructor. }
-  {econstructor. eapply f_atomicStep; eauto. constructor. }
-  {econstructor. eapply f_betaStep; eauto. constructor. }
+  {eapply c_multi_L. eapply IHc_step. inv H1. auto. }
+  {inv H1. eapply c_multi_R. eapply IHc_step. auto. }
+  {econstructor. eapply c_forkStep; eauto. constructor. }
+  {econstructor. eapply c_allocStep; eauto. constructor. }
+  {econstructor. eapply c_commitStep; eauto. constructor. }
+  {econstructor. eapply c_atomicStep; eauto. econstructor. }
+  {econstructor. eapply c_betaStep; eauto. econstructor. }
+  {econstructor. eapply c_tsExtend; eauto. constructor. }
 Qed. 
 
 (*generalize to multistep*)
@@ -75,8 +80,9 @@ Theorem partialImpliesFullMulti : forall C H T C' H' T',
 Proof.
   intros. induction H0. 
   {constructor. }
-  {copy H0. apply p_stepRewind in H0; auto. apply IHp_multistep in H0.
-   eapply partialImpliesFull in H3; eauto. eapply f_multi_trans; eauto. }
+  {copy H0. eapply p_stepRewind in H0; auto. 
+   apply IHc_multistep in H0. eapply partialImpliesFull in H3; eauto.
+   eapply c_multi_trans; eauto. }
 Qed. 
 
 
